lib/adt/BST.dfy
@@ -1,6 +1,7 @@
 include "BinaryTree.dfy"
 
 import opened BinaryTree
+import opened Seq
 
 predicate GEAll(x: int, xs: multiset<int>)   // x is >= every element (bounds a left subtree)
 {
@@ -25,4 +26,123 @@ predicate BinarySearchTree?(t: Tree<int>)
   case Nil => true
   case Node(x, l, r) =>
     GEAll(x, ToMS(l)) && LEAll(x, ToMS(r)) && BinarySearchTree?(l) && BinarySearchTree?(r)
+}
+
+lemma InorderMultiset(t: Tree<int>)
+  ensures multiset(InorderFlatten(t)) == ToMS(t)
+{
+  match t
+  case Nil =>
+  case Node(_, l, r) =>
+    InorderMultiset(l);
+    InorderMultiset(r);
+}
+
+lemma InorderMemberToMS(t: Tree<int>, x: int)
+  ensures x in InorderFlatten(t) <==> x in ToMS(t)
+{
+  InorderMultiset(t);
+}
+
+lemma BSTLeftValuesLeRoot(x: int, l: Tree<int>, r: Tree<int>)
+  requires BinarySearchTree?(Node(x, l, r))
+  ensures forall v :: v in InorderFlatten(l) ==> v <= x
+{
+  InorderMultiset(l);
+  forall v | v in InorderFlatten(l)
+    ensures v <= x
+  {
+    assert v in ToMS(l);
+  }
+}
+
+lemma BSTRightValuesGeRoot(x: int, l: Tree<int>, r: Tree<int>)
+  requires BinarySearchTree?(Node(x, l, r))
+  ensures forall v :: v in InorderFlatten(r) ==> x <= v
+{
+  InorderMultiset(r);
+  forall v | v in InorderFlatten(r)
+    ensures x <= v
+  {
+    assert v in ToMS(r);
+  }
+}
+
+lemma BSTInorderSorted(t: Tree<int>)
+  requires BinarySearchTree?(t)
+  ensures Sorted(InorderFlatten(t))
+{
+  match t
+  case Nil =>
+  case Node(x, l, r) =>
+    BSTInorderSorted(l);
+    BSTInorderSorted(r);
+    InorderMultiset(l);
+    InorderMultiset(r);
+    var lf := InorderFlatten(l);
+    var rf := InorderFlatten(r);
+    assert InorderFlatten(t) == lf + [x] + rf;
+    forall i, j | 0 <= i < j < |InorderFlatten(t)|
+      ensures InorderFlatten(t)[i] <= InorderFlatten(t)[j]
+    {
+      if j < |lf| {
+        assert lf[i] <= lf[j];
+      } else if i < |lf| {
+        assert lf[i] in lf;
+        assert lf[i] in ToMS(l);
+        if j == |lf| {
+        } else {
+          var rj := j - |lf| - 1;
+          assert 0 <= rj < |rf|;
+          assert InorderFlatten(t)[j] == rf[rj];
+          assert rf[rj] in rf;
+          assert rf[rj] in ToMS(r);
+        }
+      } else if i == |lf| {
+        if j > |lf| {
+          var rj := j - |lf| - 1;
+          assert 0 <= rj < |rf|;
+          assert InorderFlatten(t)[j] == rf[rj];
+          assert rf[rj] in rf;
+          assert rf[rj] in ToMS(r);
+        }
+      } else {
+        var ri := i - |lf| - 1;
+        var rj := j - |lf| - 1;
+        assert 0 <= ri < rj < |rf|;
+        assert rf[ri] <= rf[rj];
+      }
+    }
+}
+
+lemma BSTSearchLeftPrune(q: int, x: int, l: Tree<int>, r: Tree<int>)
+  requires BinarySearchTree?(Node(x, l, r))
+  requires q < x
+  ensures q in ToMS(Node(x, l, r)) <==> q in ToMS(l)
+{
+  if q in ToMS(Node(x, l, r)) && q !in ToMS(l) {
+    if q == x {
+      assert false;
+    } else {
+      assert q in ToMS(r);
+      assert x <= q;
+      assert false;
+    }
+  }
+}
+
+lemma BSTSearchRightPrune(q: int, x: int, l: Tree<int>, r: Tree<int>)
+  requires BinarySearchTree?(Node(x, l, r))
+  requires x < q
+  ensures q in ToMS(Node(x, l, r)) <==> q in ToMS(r)
+{
+  if q in ToMS(Node(x, l, r)) && q !in ToMS(r) {
+    if q == x {
+      assert false;
+    } else {
+      assert q in ToMS(l);
+      assert q <= x;
+      assert false;
+    }
+  }
 }
