leetcode/0001-two-sum.dfy
@@ -16,9 +16,12 @@ predicate InMap(nums: seq<int>, m: map<int, int>, t: int) {
 }
 
 method TwoSum(nums: array<int>, target: int) returns (r: (int, int))
+  ensures r.0 == -1 || 0 <= r.0
   ensures 0 <= r.0 ==> 0 <= r.0 < r.1 < nums.Length &&
                        nums[r.0] + nums[r.1] == target &&
                        forall i, j :: 0 <= i < j < r.1 ==> nums[i] + nums[j] != target
+  ensures (exists i, j :: 0 <= i < j < nums.Length && nums[i] + nums[j] == target) ==>
+            0 <= r.0 < r.1 < nums.Length && nums[r.0] + nums[r.1] == target
   ensures r.0 == -1 <==> forall i, j :: 0 <= i < j < nums.Length ==> nums[i] + nums[j] != target
 {
   var m: map<int, int> := map[];
